Simplify std/schain and std/chain.

theories/std/schain.v
@@ -28,110 +28,89 @@ Definition schain_cons : val :=
 Section zebre_G.
   Context `{zebre_G : !ZebreG Σ}.
 
-  Fixpoint schain_model node dq nodes dst : iProp Σ :=
+  Fixpoint schain_model node nodes dst : iProp Σ :=
     match nodes with
     | [] =>
         ⌜node = dst⌝
     | node' :: nodes =>
-        node.[schain_next] ↦{dq} #node' ∗
-        schain_model node' dq nodes dst
+        node.[schain_next] ↦ #node' ∗
+        schain_model node' nodes dst
     end.
-  #[global] Arguments schain_model _ _ !_ _ / : assert.
+  #[global] Arguments schain_model _ !_ _ / : assert.
 
-  #[global] Instance schain_model_timeless node dq nodes dst :
-    Timeless (schain_model node dq nodes dst).
-  Proof.
-    move: node. induction nodes; apply _.
-  Qed.
-  #[global] Instance schain_model_persistent node nodes dst :
-    Persistent (schain_model node DfracDiscarded nodes dst).
+  #[global] Instance schain_model_timeless node nodes dst :
+    Timeless (schain_model node nodes dst).
   Proof.
     move: node. induction nodes; apply _.
   Qed.
 
-  #[global] Instance schain_model_fractional node nodes dst :
-    Fractional (λ q, schain_model node (DfracOwn q) nodes dst).
-  Proof.
-    intros q1 q2.
-    move: node. induction nodes as [| node' nodes IH] => node /=; first iSteps.
-    setoid_rewrite IH. setoid_rewrite pointsto_fractional.
-    iSplit.
-    - iIntros "((Hnode1 & Hnode2) & (Hnode'1 & Hnode'2))". iSteps.
-    - iIntros "((Hnode1 & Hnode'1) & (Hnode2 & Hnode'2))". iSteps.
-  Qed.
-  #[global] Instance schain_model_as_fractional node q nodes dst :
-    AsFractional (schain_model node (DfracOwn q) nodes dst) (λ q, schain_model node (DfracOwn q) nodes dst) q.
-  Proof.
-    split; [done | apply _].
-  Qed.
-
-  Lemma schain_model_nil node dq dst :
+  Lemma schain_model_nil node dst :
     ⌜node = dst⌝ ⊣⊢
-    schain_model node dq [] dst.
+    schain_model node [] dst.
   Proof.
     iSteps.
   Qed.
-  Lemma schain_model_nil_1 node dq :
-    ⊢ schain_model node dq [] node.
+  Lemma schain_model_nil_1 node :
+    ⊢ schain_model node [] node.
   Proof.
     iSteps.
   Qed.
-  Lemma schain_model_nil_2 node dq dst :
-    schain_model node dq [] dst ⊢
+  Lemma schain_model_nil_2 node dst :
+    schain_model node [] dst ⊢
     ⌜node = dst⌝.
   Proof.
     iSteps.
   Qed.
 
-  Lemma schain_model_cons node dq nodes node' nodes' dst :
+  Lemma schain_model_cons node nodes node' nodes' dst :
     nodes = node' :: nodes' →
-    schain_model node dq nodes dst ⊣⊢
-      node.[schain_next] ↦{dq} #node' ∗
-      schain_model node' dq nodes' dst.
+    schain_model node nodes dst ⊣⊢
+      node.[schain_next] ↦ #node' ∗
+      schain_model node' nodes' dst.
   Proof.
     iSteps.
   Qed.
-  Lemma schain_model_cons_1 node dq nodes node' nodes' dst :
+  Lemma schain_model_cons_1 node nodes node' nodes' dst :
     nodes = node' :: nodes' →
-    schain_model node dq nodes dst ⊢
-      node.[schain_next] ↦{dq} #node' ∗
-      schain_model node' dq nodes' dst.
+    schain_model node nodes dst ⊢
+      node.[schain_next] ↦ #node' ∗
+      schain_model node' nodes' dst.
   Proof.
     iSteps.
   Qed.
-  Lemma schain_model_cons_2 node dq node' nodes dst :
-    node.[schain_next] ↦{dq} #node' -∗
-    schain_model node' dq nodes dst -∗
-    schain_model node dq (node' :: nodes) dst.
+  Lemma schain_model_cons_2 node node' nodes dst :
+    node.[schain_next] ↦ #node' -∗
+    schain_model node' nodes dst -∗
+    schain_model node (node' :: nodes) dst.
   Proof.
     iSteps.
   Qed.
 
-  Lemma schain_model_app_1 dq node1 nodes1 node2 nodes2 dst :
-    schain_model node1 dq nodes1 node2 -∗
-    schain_model node2 dq nodes2 dst -∗
-    schain_model node1 dq (nodes1 ++ nodes2) dst.
+  Lemma schain_model_app_1 node1 nodes1 node2 nodes2 dst :
+    schain_model node1 nodes1 node2 -∗
+    schain_model node2 nodes2 dst -∗
+    schain_model node1 (nodes1 ++ nodes2) dst.
   Proof.
     iInduction nodes1 as [| node1' nodes1] "IH" forall (node1); iSteps.
   Qed.
-  Lemma schain_model_app_2 nodes1 nodes2 node dq nodes dst :
+  Lemma schain_model_app_2 nodes1 nodes2 node nodes dst :
     nodes = nodes1 ++ nodes2 →
-    schain_model node dq nodes dst ⊢
+    schain_model node nodes dst ⊢
       ∃ node',
-      schain_model node dq nodes1 node' ∗
-      schain_model node' dq nodes2 dst.
+      schain_model node nodes1 node' ∗
+      schain_model node' nodes2 dst.
   Proof.
     iInduction nodes1 as [| node1 nodes1] "IH" forall (node nodes); first iSteps.
     iIntros (->). rewrite -app_comm_cons. iIntros "(Hnode & Hnode1)".
     iDestruct ("IH" with "[//] Hnode1") as "(%node' & Hnode1 & Hnode')".
     iSteps.
   Qed.
-  Lemma schain_model_app node dq nodes1 nodes2 dst :
+  Lemma schain_model_app node nodes1 nodes2 dst :
     ( ∃ node',
-      schain_model node dq nodes1 node' ∗
-      schain_model node' dq nodes2 dst
+      schain_model node nodes1 node' ∗
+      schain_model node' nodes2 dst
     ) ⊣⊢
-    schain_model node dq (nodes1 ++ nodes2) dst.
+    schain_model node (nodes1 ++ nodes2) dst.
   Proof.
     iSplit.
     - iIntros "(%node' & Hnode & Hnode')".
@@ -139,153 +118,43 @@ Section zebre_G.
     - iApply schain_model_app_2; first done.
   Qed.
 
-  Lemma schain_model_valid node dq nodes dst :
-    0 < length nodes →
-    schain_model node dq nodes dst ⊢
-    ⌜✓ dq⌝.
-  Proof.
-    intros Hlen. destruct nodes as [| node' nodes]; first naive_solver lia.
-    iIntros "(Hnode & _)".
-    iApply (pointsto_valid with "Hnode").
-  Qed.
-  Lemma schain_model_combine node dq1 nodes1 dst1 dq2 nodes2 dst2 :
-    length nodes1 ≤ length nodes2 →
-    schain_model node dq1 nodes1 dst1 -∗
-    schain_model node dq2 nodes2 dst2 -∗
-      schain_model node (dq1 ⋅ dq2) nodes1 dst1 ∗
-      schain_model dst1 dq2 (drop (length nodes1) nodes2) dst2 ∗
-      ⌜nodes1 = take (length nodes1) nodes2⌝.
-  Proof.
-    iInduction nodes1 as [| node1' nodes1] "IH" forall (node nodes2); first iSteps.
-    destruct nodes2 as [| node2' nodes2].
-    - iSteps. lia.
-    - iIntros "%Hlen (Hnode_1 & Hnode1') (Hnode_2 & Hnode2')".
-      simpl in Hlen. apply le_S_n in Hlen.
-      iDestruct (pointsto_combine with "Hnode_1 Hnode_2") as "(Hnode & %Heq)". injection Heq as <-.
-      iDestruct ("IH" with "[] Hnode1' Hnode2'") as "(Hnode1' & Hdst1 & ->)"; first done.
-      rewrite /= take_length min_l //. iSteps.
-  Qed.
-  Lemma schain_model_combine' node dq1 nodes1 dst1 dq2 nodes2 dst2 :
-    length nodes1 = length nodes2 →
-    schain_model node dq1 nodes1 dst1 -∗
-    schain_model node dq2 nodes2 dst2 -∗
-      schain_model node (dq1 ⋅ dq2) nodes1 dst1 ∗
-      ⌜nodes1 = nodes2 ∧ dst1 = dst2⌝.
-  Proof.
-    iIntros "%Hlen Hnode_1 Hnode_2".
-    iDestruct (schain_model_combine with "Hnode_1 Hnode_2") as "($ & Hdst1 & ->)"; first lia.
-    rewrite Hlen take_length min_l; first lia.
-    rewrite drop_all. iDestruct "Hdst1" as %->.
-    rewrite take_ge //.
-  Qed.
-  Lemma schain_model_valid_2 node dq1 nodes1 dst1 dq2 nodes2 dst2 :
-    0 < length nodes1 ≤ length nodes2 →
-    schain_model node dq1 nodes1 dst1 -∗
-    schain_model node dq2 nodes2 dst2 -∗
-    ⌜✓ (dq1 ⋅ dq2) ∧ nodes1 = take (length nodes1) nodes2⌝.
-  Proof.
-    iIntros "% Hnode_1 Hnode_2".
-    iDestruct (schain_model_combine with "Hnode_1 Hnode_2") as "(Hnode & _ & %)"; first lia.
-    iDestruct (schain_model_valid with "Hnode") as %?; first lia.
-    iSteps.
-  Qed.
-  Lemma schain_model_valid_2' node dq1 nodes1 dst1 dq2 nodes2 dst2 :
-    0 < length nodes1 →
-    length nodes1 = length nodes2 →
-    schain_model node dq1 nodes1 dst1 -∗
-    schain_model node dq2 nodes2 dst2 -∗
-    ⌜✓ (dq1 ⋅ dq2) ∧ nodes1 = nodes2 ∧ dst1 = dst2⌝.
-  Proof.
-    iIntros "% % Hnode_1 Hnode_2".
-    iDestruct (schain_model_combine' with "Hnode_1 Hnode_2") as "(Hnode & <- & <-)"; first done.
-    iDestruct (schain_model_valid with "Hnode") as %?; first done.
-    iSteps.
-  Qed.
-  Lemma schain_model_agree node dq1 nodes1 dst1 dq2 nodes2 dst2 :
-    length nodes1 = length nodes2 →
-    schain_model node dq1 nodes1 dst1 -∗
-    schain_model node dq2 nodes2 dst2 -∗
-    ⌜nodes1 = nodes2 ∧ dst1 = dst2⌝.
-  Proof.
-    iIntros "% Hnode_1 Hnode_2".
-    iDestruct (schain_model_combine' with "Hnode_1 Hnode_2") as "(_ & <- & <-)"; first done.
-    iSteps.
-  Qed.
-  Lemma schain_model_dfrac_ne node1 dq1 nodes1 dst1 node2 dq2 nodes2 dst2 :
-    0 < length nodes1 →
-    0 < length nodes2 →
-    ¬ ✓ (dq1 ⋅ dq2) →
-    schain_model node1 dq1 nodes1 dst1 -∗
-    schain_model node2 dq2 nodes2 dst2 -∗
-    ⌜node1 ≠ node2⌝.
-  Proof.
-    intros. destruct nodes1, nodes2; [naive_solver lia.. |].
-    iIntros "(Hnode1 & _) (Hnode2 & _) <-".
-    iCombine "Hnode1 Hnode2" gives %(? & _). done.
-  Qed.
-  Lemma schain_model_ne node1 nodes1 dst1 node2 dq2 nodes2 dst2 :
-    0 < length nodes1 →
-    0 < length nodes2 →
-    schain_model node1 (DfracOwn 1) nodes1 dst1 -∗
-    schain_model node2 dq2 nodes2 dst2 -∗
-    ⌜node1 ≠ node2⌝.
-  Proof.
-    intros.
-    iApply schain_model_dfrac_ne; [done.. | intros []%exclusive_l; apply _].
-  Qed.
   Lemma schain_model_exclusive node nodes1 dst1 nodes2 dst2 :
     0 < length nodes1 →
     0 < length nodes2 →
-    schain_model node (DfracOwn 1) nodes1 dst1 -∗
-    schain_model node (DfracOwn 1) nodes2 dst2 -∗
+    schain_model node nodes1 dst1 -∗
+    schain_model node nodes2 dst2 -∗
     False.
   Proof.
-    iIntros "% % Hnode_1 Hnode_2".
-    iDestruct (schain_model_ne with "Hnode_1 Hnode_2") as %?; done.
-  Qed.
-  Lemma schain_model_persist node dq nodes dst :
-    schain_model node dq nodes dst ⊢ |==>
-    schain_model node DfracDiscarded nodes dst.
-  Proof.
-    iInduction nodes as [] "IH" forall (node); iSteps.
+    intros.
+    destruct nodes1, nodes2; [naive_solver lia.. |].
+    iIntros "(Hnode1 & _) (Hnode2 & _)".
+    iCombine "Hnode1 Hnode2" gives %(? & _). done.
   Qed.
 
-  Lemma schain_cons_spec node dq nodes dst v :
+  Lemma schain_cons_spec node nodes dst v :
     {{{
-      schain_model node dq nodes dst
+      schain_model node nodes dst
     }}}
       schain_cons v #node
     {{{ node',
       RET #node';
       node'.[schain_data] ↦ v ∗
-      schain_model node' (DfracOwn 1) [node] node ∗
-      schain_model node dq nodes dst
-    }}}.
-  Proof.
-    iSteps.
-  Qed.
-  Lemma schain_cons_spec_raw v1 v2 :
-    {{{ True }}}
-      schain_cons v1 v2
-    {{{ node,
-      RET #node;
-      node.[schain_data] ↦ v1 ∗
-      node.[schain_next] ↦ v2
+      schain_model node' (node :: nodes) dst
     }}}.
   Proof.
     iSteps.
   Qed.
 
-  Lemma schain_next_spec {node dq nodes} node' nodes' dst :
+  Lemma schain_next_spec {node nodes} node' nodes' dst :
     nodes = node' :: nodes' →
     {{{
-      schain_model node dq nodes dst
+      schain_model node nodes dst
     }}}
       (#node).{schain_next}
     {{{
       RET #node';
-      schain_model node dq [node'] node' ∗
-      schain_model node' dq nodes' dst
+      schain_model node [node'] node' ∗
+      schain_model node' nodes' dst
     }}}.
   Proof.
     iSteps.
@@ -294,13 +163,13 @@ Section zebre_G.
   Lemma schain_set_next_spec {node nodes} node' nodes' dst l :
     nodes = node' :: nodes' →
     {{{
-      schain_model node (DfracOwn 1) nodes dst
+      schain_model node nodes dst
     }}}
       #node <-{schain_next} #l
     {{{
       RET ();
-      schain_model node (DfracOwn 1) [l] l ∗
-      schain_model node' (DfracOwn 1) nodes' dst
+      schain_model node [l] l ∗
+      schain_model node' nodes' dst
     }}}.
   Proof.
     iSteps.
